updated mapsto_memory_block

veric/Clight_seplog.v
@@ -1,8 +1,4 @@
-Require Import VST.msl.log_normalize.
-Require Import VST.msl.alg_seplog.
 Require Export VST.veric.base.
-Require Import VST.veric.rmaps.
-Require Import VST.veric.compcert_rmaps.
 Require Import VST.veric.res_predicates.
 
 Require Import VST.veric.mpred.
@@ -13,16 +9,11 @@ Require Export VST.veric.seplog.
 
 Require Export VST.veric.mapsto_memory_block.
 
-Local Open Scope pred.
-
-Require Import compcert.cfrontend.Clight. 
+Require Import compcert.cfrontend.Clight.
 Require Import VST.veric.tycontext.
 Require Import VST.veric.expr2.
 Require Import VST.veric.binop_lemmas2.
 Require Export VST.veric.Clight_mapsto_memory_block.
-Import compcert.lib.Maps.
-
-Local Open Scope pred.
 
 Definition mkEnv g ids vals : environ := 
       let n := Nat.min (length ids) (length vals) in
@@ -42,30 +33,32 @@ Definition eval_lvar (id: ident) (ty: type) (rho: environ) :=
 | None => Vundef
 end.
 
+Section mpred.
+
+Context `{!heapGS Σ}.
+
 Definition var_block (sh: Share.t) {cs: compspecs} (idt: ident * type) (rho: environ): mpred :=
-  !! (sizeof (snd idt) <= Ptrofs.max_unsigned) &&
+  ⌜sizeof (snd idt) <= Ptrofs.max_unsigned⌝ ∧
   (memory_block sh (sizeof (snd idt))) (eval_lvar (fst idt) (snd idt) rho).
 
-Definition stackframe_of {cs: compspecs} (f: Clight.function) : assert :=
-  fold_right (fun P Q rho => P rho * Q rho) (fun rho => emp) (map (fun idt => var_block Share.top idt) (Clight.fn_vars f)).
+Definition stackframe_of {cs: compspecs} (f: Clight.function) : environ -> mpred :=
+  fold_right (fun P Q rho => P rho ∗ Q rho) (fun rho => emp) (map (fun idt => var_block Share.top idt) (Clight.fn_vars f)).
 
 Lemma stackframe_of_eq : forall {cs: compspecs}, stackframe_of =
-        fun f rho => fold_right sepcon emp (map (fun idt => var_block Share.top idt rho) (Clight.fn_vars f)).
+        fun f rho => fold_right bi_sep emp (map (fun idt => var_block Share.top idt rho) (Clight.fn_vars f)).
 Proof.
   intros.
- extensionality f rho.
- unfold stackframe_of.
- forget (fn_vars f) as vl.
- induction vl; simpl; auto.
- rewrite IHvl; auto.
+  extensionality f rho.
+  unfold stackframe_of.
+  forget (fn_vars f) as vl.
+  induction vl; simpl; auto.
+  rewrite IHvl; auto.
 Qed.
 
 Lemma  subst_derives:
- forall a v P Q, (forall rho, P rho |-- Q rho) -> forall rho, subst a v P rho |-- subst a v Q rho.
+ forall a v (P Q : environ -> mpred), (forall rho, P rho ⊢ Q rho) -> forall rho, subst a v P rho ⊢ subst a v Q rho.
 Proof.
-unfold subst, derives.
-simpl;
-auto.
+  exact subst_extens.
 Qed.
 
 Definition tc_formals (formals: list (ident * type)) : environ -> Prop :=
@@ -75,52 +68,52 @@ Definition tc_formals (formals: list (ident * type)) : environ -> Prop :=
 
 Definition close_precondition (bodyparams: list ident) 
     (P: argsEnviron -> mpred) (rho:environ) : mpred :=
- EX vals,
-   !!(map (Map.get (te_of rho)) bodyparams = map Some vals /\
-      Forall (fun v : val => v <> Vundef) vals) &&
+ ∃ vals,
+   ⌜map (Map.get (te_of rho)) bodyparams = map Some vals /\
+      Forall (fun v : val => v <> Vundef) vals⌝ ∧
    P (ge_of rho, vals).
 
-Definition precondition_closed (fs: list (ident*type)) {A: TypeTree}
-  (P: forall ts, dependent_type_functor_rec ts (AssertTT A) mpred) : Prop :=
- forall ts x,
-  closed_wrt_vars (not_a_param fs) (P ts x) /\
-  closed_wrt_lvars (fun _ => True) (P ts x).
+Definition precondition_closed (fs: list (ident*type)) {A}
+  (P: A -> environ -> mpred) : Prop :=
+ forall x,
+  closed_wrt_vars (not_a_param fs) (P x) /\
+  closed_wrt_lvars (fun _ => True%type) (P x).
 
 Lemma close_precondition_e':
-   forall al (P: argsEnviron -> pred rmap) (rho: environ) ,
-   close_precondition al P rho |-- 
-   exp (fun vals =>
-     !!(map (Map.get (te_of rho)) al = map Some vals/\
-        Forall (fun v : val => v <> Vundef) vals) &&
-   P (ge_of rho, vals)).
-Proof. intros. intros u p. simpl in p. simpl; trivial. Qed.
+   forall al (P: argsEnviron -> mpred) (rho: environ),
+   close_precondition al P rho ⊢ 
+   ∃ vals,
+     ⌜map (Map.get (te_of rho)) al = map Some vals /\
+        Forall (fun v : val => v <> Vundef) vals⌝ ∧
+   P (ge_of rho, vals).
+Proof. trivial. Qed.
 
 Lemma Forall_eval_id_get: forall {vals: list val} (V:Forall (fun v : val => v = Vundef -> False) vals), 
   forall ids rho, map (Map.get (te_of rho)) ids = map Some vals <-> map (fun i : ident => eval_id i rho) ids = vals.
 Proof.
 induction vals; simpl; intros; split; intros; destruct ids; inv H; simpl in *; trivial.
 + inv V. destruct (IHvals H4 ids rho) as [X _]. rewrite (X H2); clear X H2. f_equal.
-  unfold eval_id; rewrite H1; simpl; trivial. 
+  unfold eval_id; rewrite H1; simpl; trivial.
 + inv V. destruct (IHvals H2 ids rho) as [_ X]. rewrite X; clear X; trivial. f_equal.
   clear - H1. unfold eval_id, force_val in *.
   destruct (Map.get (te_of rho) p); trivial. elim H1; trivial.
 Qed.
 
 Lemma close_precondition_eval_id ids P rho:
-   close_precondition ids P rho = 
-   EX vals:_,
-     !!(map (fun i => eval_id i rho) ids = vals /\
-        Forall (fun v : val => v <> Vundef) vals) &&
+   close_precondition ids P rho ⊣⊢
+   ∃ vals:_,
+     ⌜map (fun i => eval_id i rho) ids = vals /\
+        Forall (fun v : val => v <> Vundef) vals⌝ ∧
    P (ge_of rho, vals).
 Proof.
-unfold close_precondition. apply pred_ext; apply exp_derives; intros vals m M; simpl in *; intuition.
-apply (Forall_eval_id_get H2); trivial.
-apply (Forall_eval_id_get H2); trivial.
-Qed.
+unfold close_precondition.
+apply bi.exist_proper; intros vals; apply bi.and_proper; last done; apply bi.pure_proper; intuition;
+  apply (Forall_eval_id_get); trivial.
+Qed. 
 
-Definition bind_args (bodyparams: list (ident * type)) (P: genviron * list val -> pred rmap) : assert :=
-  fun rho => !! tc_formals bodyparams rho 
-     && close_precondition (map fst bodyparams) P rho.
+Definition bind_args (bodyparams: list (ident * type)) (P: genviron * list val -> mpred) : environ -> mpred :=
+  fun rho => ⌜tc_formals bodyparams rho⌝
+     ∧ close_precondition (map fst bodyparams) P rho.
 
 Definition ret_temp : ident := 1%positive.
 
@@ -133,12 +126,12 @@ Definition get_result (ret: option ident) : environ -> environ :=
  | Some x => get_result1 x
  end.
 
-Definition bind_ret (vl: option val) (t: type) (Q: assert) : assert :=
+Definition bind_ret (vl: option val) (t: type) (Q: environ -> mpred) : environ -> mpred :=
      match vl, t with
      | None, Tvoid => fun rho => Q (make_args nil nil rho)
-     | Some v, _ => fun rho => !! (tc_val t v) &&
+     | Some v, _ => fun rho => ⌜tc_val t v⌝ ∧
                                Q (make_args (ret_temp::nil) (v::nil) rho)
-     | _, _ => fun rho => FF
+     | _, _ => fun rho => False
      end.
 
 Definition funassert (Delta: tycontext): assert := funspecs_assert (glob_specs Delta).
@@ -149,109 +142,115 @@ Definition funassert (Delta: tycontext): assert := funspecs_assert (glob_specs D
   using different shares that don't have a common core, whereas address_mapsto
   requires the same share on all four bytes. *)
 
-Definition proj_ret_assert (Q: ret_assert) (ek: exitkind) (vl: option val) : assert :=
+Definition proj_ret_assert (Q: ret_assert) (ek: exitkind) (vl: option val) : environ -> mpred :=
  match ek with
- | EK_normal => fun rho => !! (vl=None) && RA_normal Q rho
- | EK_break => fun rho => !! (vl=None) && RA_break Q rho
- | EK_continue => fun rho => !! (vl=None) && RA_continue Q rho
+ | EK_normal => fun rho => ⌜vl=None⌝ ∧ RA_normal Q rho
+ | EK_break => fun rho => ⌜vl=None⌝ ∧ RA_break Q rho
+ | EK_continue => fun rho => ⌜vl=None⌝ ∧ RA_continue Q rho
  | EK_return => RA_return Q vl
  end.
 
-Definition overridePost  (Q: assert)  (R: ret_assert) :=
+Definition overridePost  (Q: environ -> mpred)  (R: ret_assert) :=
  match R with 
   {| RA_normal := _; RA_break := b; RA_continue := c; RA_return := r |} =>
   {| RA_normal := Q; RA_break := b; RA_continue := c; RA_return := r |}
  end.
 
 Definition existential_ret_assert {A: Type} (R: A -> ret_assert) :=
-  {| RA_normal := fun rho => EX x:A, (R x).(RA_normal) rho;
-     RA_break := fun rho => EX x:A, (R x).(RA_break) rho;
-     RA_continue := fun rho => EX x:A, (R x).(RA_continue) rho;
-     RA_return := fun vl rho => EX x:A, (R x).(RA_return) vl rho
+  {| RA_normal := fun rho => ∃ x:A, (R x).(RA_normal) rho;
+     RA_break := fun rho => ∃ x:A, (R x).(RA_break) rho;
+     RA_continue := fun rho => ∃ x:A, (R x).(RA_continue) rho;
+     RA_return := fun vl rho => ∃ x:A, (R x).(RA_return) vl rho
    |}.
 
-Definition normal_ret_assert (Q: assert) : ret_assert :=
-  {| RA_normal := Q; RA_break := seplog.FF; RA_continue := seplog.FF; RA_return := fun _ => seplog.FF |}.
+Definition normal_ret_assert (Q: environ -> mpred) : ret_assert :=
+  {| RA_normal := Q; RA_break _ := False; RA_continue _ := False; RA_return _ := fun _ => False |}.
 
-Definition frame_ret_assert (R: ret_assert) (F: assert) : ret_assert :=
+Definition frame_ret_assert (R: ret_assert) (F: environ -> mpred) : ret_assert :=
  match R with 
   {| RA_normal := n; RA_break := b; RA_continue := c; RA_return := r |} =>
-  {| RA_normal := fun rho => n rho * F rho; 
-     RA_break := fun rho => b rho * F rho; 
-     RA_continue := fun rho => c rho * F rho;
-     RA_return := fun vl rho => r vl rho * F rho |}
+  {| RA_normal := fun rho => n rho ∗ F rho; 
+     RA_break := fun rho => b rho ∗ F rho; 
+     RA_continue := fun rho => c rho ∗ F rho;
+     RA_return := fun vl rho => r vl rho ∗ F rho |}
  end.
 
-Definition conj_ret_assert (R: ret_assert) (F: assert) : ret_assert :=
+Definition conj_ret_assert (R: ret_assert) (F: environ -> mpred) : ret_assert :=
  match R with 
   {| RA_normal := n; RA_break := b; RA_continue := c; RA_return := r |} =>
-  {| RA_normal := fun rho => n rho && F rho; 
-     RA_break := fun rho => b rho && F rho; 
-     RA_continue := fun rho => c rho && F rho;
-     RA_return := fun vl rho => r vl rho && F rho |}
+  {| RA_normal := fun rho => n rho ∧ F rho; 
+     RA_break := fun rho => b rho ∧ F rho; 
+     RA_continue := fun rho => c rho ∧ F rho;
+     RA_return := fun vl rho => r vl rho ∧ F rho |}
  end.
 
 Definition switch_ret_assert (R: ret_assert) : ret_assert :=
  match R with 
   {| RA_normal := n; RA_break := b; RA_continue := c; RA_return := r |} =>
-  {| RA_normal := seplog.FF; 
+  {| RA_normal _ := False; 
      RA_break := n; 
      RA_continue := c;
      RA_return := r |}
  end.
 
-Require Import VST.msl.normalize.
-
 Lemma normal_ret_assert_derives:
  forall P Q rho,
-  (P rho |-- Q rho) ->
+  (P rho ⊢ Q rho) ->
   forall ek vl, proj_ret_assert (normal_ret_assert P) ek vl rho 
-            |-- proj_ret_assert (normal_ret_assert Q) ek vl rho.
+            ⊢ proj_ret_assert (normal_ret_assert Q) ek vl rho.
 Proof.
- intros.
- destruct ek; simpl; normalize.
+  intros.
+  destruct ek; simpl; auto.
+  by rewrite H.
 Qed.
-#[export] Hint Resolve normal_ret_assert_derives : core.
 
-Lemma normal_ret_assert_FF:
-  forall ek vl rho, proj_ret_assert (normal_ret_assert (fun rho => FF)) ek vl rho = FF.
+Lemma normal_ret_assert_False:
+  forall ek vl rho, proj_ret_assert (normal_ret_assert (fun rho => False)) ek vl rho ⊣⊢ False.
 Proof.
 intros.
-destruct ek; simpl; normalize.
+destruct ek; simpl; auto; by rewrite bi.and_False.
 Qed.
+
+(* Do we care about the kind of equivalence? Should this be an assert? *)
+Global Instance ret_assert_equiv : Equiv ret_assert := fun a b =>
+  (forall e, RA_normal a e ⊣⊢ RA_normal b e) /\ (forall e, RA_break a e ⊣⊢ RA_break b e) /\
+  (forall e, RA_continue a e ⊣⊢ RA_continue b e) /\ (forall v e, RA_return a v e ⊣⊢ RA_return b v e).
 
 Lemma frame_normal:
   forall P F,
-   frame_ret_assert (normal_ret_assert P) F = normal_ret_assert (fun rho => P rho * F rho).
+   ret_assert_equiv (frame_ret_assert (normal_ret_assert P) F) (normal_ret_assert (fun rho => P rho ∗ F rho)).
 Proof.
 intros.
 unfold normal_ret_assert; simpl.
-f_equal; simpl; try solve [extensionality rho; normalize].
-extensionality vl rho; normalize.
+split3; last split; simpl; auto; intros; by rewrite bi.sep_False.
+Qed.
+
+Lemma pure_and_sep_assoc: forall P (Q R : mpred), ⌜P⌝ ∧ Q ∗ R ⊣⊢ (⌜P⌝ ∧ Q) ∗ R.
+Proof.
+  intros; iSplit.
+  - iIntros "($ & $ & $)".
+  - iIntros "(($ & $) & $)".
 Qed.
 
 Lemma proj_frame:
-  forall P F ek vl,
-    proj_ret_assert (frame_ret_assert P F) ek vl = fun rho => F rho * proj_ret_assert P ek vl rho.
+  forall P F ek vl rho,
+    proj_ret_assert (frame_ret_assert P F) ek vl rho ⊣⊢ F rho ∗ proj_ret_assert P ek vl rho.
 Proof.
   intros.
-  extensionality rho.
-  rewrite sepcon_comm.
-  destruct ek; simpl; destruct P; auto;
-  normalize.
+  rewrite bi.sep_comm.
+  destruct ek; simpl; destruct P; auto; simpl; apply pure_and_sep_assoc.
 Qed.
 
 Lemma proj_conj:
-  forall P F ek vl,
-    proj_ret_assert (conj_ret_assert P F) ek vl = fun rho => F rho && proj_ret_assert P ek vl rho.
+  forall P F ek vl rho,
+    proj_ret_assert (conj_ret_assert P F) ek vl rho ⊣⊢ F rho ∧ proj_ret_assert P ek vl rho.
 Proof.
   intros.
-  extensionality rho.
-  rewrite andp_comm.
-  destruct ek; simpl; destruct P; auto; simpl; normalize; rewrite andp_assoc; auto.
+  rewrite bi.and_comm.
+  destruct ek; simpl; destruct P; auto; simpl; by rewrite assoc.
 Qed.
 
-Definition loop1_ret_assert (Inv: assert) (R: ret_assert) : ret_assert :=
+Definition loop1_ret_assert (Inv: environ -> mpred) (R: ret_assert) : ret_assert :=
  match R with 
   {| RA_normal := n; RA_break := b; RA_continue := c; RA_return := r |} =>
   {| RA_normal := Inv;
@@ -260,19 +259,19 @@ Definition loop1_ret_assert (Inv: assert) (R: ret_assert) : ret_assert :=
      RA_return := r |}
  end.
 
-Definition loop2_ret_assert (Inv: assert) (R: ret_assert) : ret_assert :=
+Definition loop2_ret_assert (Inv: environ -> mpred) (R: ret_assert) : ret_assert :=
  match R with 
   {| RA_normal := n; RA_break := b; RA_continue := c; RA_return := r |} =>
   {| RA_normal := Inv;
      RA_break := n;
-     RA_continue := seplog.FF;
+     RA_continue _ := False;
      RA_return := r |}
  end.
 
 Lemma frame_for1:
   forall Q R F,
    frame_ret_assert (loop1_ret_assert Q R) F =
-   loop1_ret_assert (fun rho => Q rho * F rho) (frame_ret_assert R F).
+   loop1_ret_assert (fun rho => Q rho ∗ F rho) (frame_ret_assert R F).
 Proof.
 intros.
 destruct R; simpl; auto.
@@ -280,12 +279,13 @@ Qed.
 
 Lemma frame_loop1:
   forall Q R F,
-   frame_ret_assert (loop2_ret_assert Q R) F =
-   loop2_ret_assert (fun rho => Q rho * F rho) (frame_ret_assert R F).
+   ret_assert_equiv (frame_ret_assert (loop2_ret_assert Q R) F)
+   (loop2_ret_assert (fun rho => Q rho ∗ F rho) (frame_ret_assert R F)).
 Proof.
 intros.
-destruct R; simpl; auto.
-f_equal; extensionality; normalize.
+destruct R; unfold ret_assert_equiv; simpl.
+split3; last split; auto.
+intros; by rewrite bi.sep_False.
 Qed.
 
 Lemma overridePost_normal:
@@ -295,17 +295,20 @@ intros; unfold overridePost, normal_ret_assert.
 f_equal.
 Qed.
 
-#[export] Hint Rewrite normal_ret_assert_FF frame_normal frame_for1 frame_loop1
-                 overridePost_normal: normalize.
-
 Definition function_body_ret_assert (ret: type) (Q: assert) : ret_assert :=
  {| RA_normal := bind_ret None ret Q;
-    RA_break := seplog.FF; 
-    RA_continue := seplog.FF;
+    RA_break _ := False; 
+    RA_continue _ := False;
     RA_return := fun vl => bind_ret vl ret Q |}.
 
 Lemma same_glob_funassert:
   forall Delta1 Delta2,
-     (forall id, (glob_specs Delta1) ! id = (glob_specs Delta2) ! id) ->
-              funassert Delta1 = funassert Delta2.
+     (forall id, (glob_specs Delta1) !! id = (glob_specs Delta2) !! id) ->
+              funassert Delta1 ⊣⊢ funassert Delta2.
 Proof. intros; eapply same_FS_funspecs_assert; trivial. Qed.
+
+End mpred.
+
+#[export] Hint Resolve normal_ret_assert_derives : core.
+(*#[export] Hint Rewrite normal_ret_assert_False frame_normal frame_for1 frame_loop1
+                 overridePost_normal: normalize.*)
